\documentclass{article}

\usepackage[utf8]{inputenc}
\usepackage[english]{babel}
\usepackage{amsmath, amssymb, gensymb}

\usepackage{graphicx}
\usepackage{fancyhdr}
\usepackage{tabularx}

\begin{document}
%-------------------------------------------------------------------------------
\section*{Exercise 1}
\begin{itemize}
\item[IH:] (induction hypothesis)
  \begin{displaymath}
    \sum_{i=1}^{n}i = \frac{n(n+1)}{2}
  \end{displaymath}
\item[IB:] $n := 1$ (induction base)
  \begin{displaymath}
    \sum_{i=1}^{n} i = \sum_{i=1}^{1} i = 1
    = \frac{1 \cdot (1 + 1)}{2} = \frac{n \cdot (n+1)}{2}
  \end{displaymath}
\item[IS:] $n := n + 1$ (induction step)
  \begin{align*}
    \sum_{i=1}^{n+1} i &= (n + 1) + \sum_{i=1}^{n} i\\
    {} &\stackrel{IH}{=} (n + 1) + \frac{n \cdot (n + 1)}{2}\\
    {} &= \frac{2 \cdot (n + 1)}{2} + \frac{n \cdot (n + 1)}{2}\\
% Uncomment for sub-transformations
%    {} &= 2 \cdot \frac{(n + 1)}{2} + n \cdot \frac{(n + 1)}{2}\\
%    {} &= (n + 2) \cdot \frac{(n + 1)}{2}\\
    {} &= \frac{(n + 2) \cdot (n + 1)}{2}\\
    {} &= \frac{((n + 1) + 1) \cdot (n + 1)}{2}
  \end{align*}
\end{itemize}
\pagebreak
%-------------------------------------------------------------------------------
\section*{Exercise 2}
\begin{itemize}
  \item[IH:] (induction hypothesis)
  \begin{displaymath}
    \sum_{i=1}^{d} \left(2^{d - i} \cdot i\right) \leq 2^{d + 1} - d - 2
  \end{displaymath}
  \item[IB:] $d := 1$ (induction base)
  \begin{displaymath}
    \sum_{i=1}^{d} \left(2^{d - i} \cdot i\right) = 2^0 \cdot 1 = 1
    \leq 1 = 2^2 - 1 - 2 = 2^{d + 1} - d - 2
  \end{displaymath}
  \item[IS:] $d := d + 1$ (induction step)
  \begin{align*}
    \sum_{i=1}^{d + 1} \left(2^{(d + 1) - i} \cdot i\right)
    &= 2 \cdot \sum_{i=1}^{d + 1} \left(2^{d - i} \cdot i\right)\\
    {} &=
      2 \cdot \sum_{i=1}^{d} \left(2^{d - i} \cdot i\right)
      + 2 \cdot \left(2^{d - (d + 1)} \cdot (d + 1)\right)\\
    {} &= 2 \cdot \sum_{i=1}^{d} \left(2^{d - i} \cdot i\right)
      + 2 \cdot \left(2^{-1} \cdot (d + 1)\right)\\
    {} &= 2 \cdot \sum_{i=1}^{d} \left(2^{d - i} \cdot i\right)
      + (d + 1)\\
    {} & \stackrel{IH}{\leq}
      2 \cdot \left(2^{d + 1} - d - 2\right) + (d + 1)\\
    {} & \hspace{1.5em} = 2^{(d + 1) + 1} - 2d - 4 + d + 1\\
    {} & \hspace{1.5em} = 2^{(d + 1) + 1} - d - 3\\
    {} & \hspace{1.5em} = 2^{(d + 1) + 1} - (d + 1) - 2
  \end{align*}
\end{itemize}
\end{document}